Alg/Nat/PrimeFactors/Union.lean
@@ -2,15 +2,30 @@ import Alg.Nat.PrimeFactors.Difference
 import Alg.Nat.PrimeFactors.Sublist
 import Alg.Nat.PrimeFactors.Intersect
 import Alg.Nat.PrimeFactors.Merge
+import Alg.ListProps.Sorted.SetOps
 import Alg.Nat.Lcm
 
-def PrimeFactors.union
+def PrimeFactorization.union
   (pa: PrimeFactorization a)
   (pb: PrimeFactorization b):
   PrimeFactorization (nat.lcm a b) := by
   unfold nat.lcm
-  have pa_mul_b := pa.merge pb
-  have pa_gcd_b := pa.intersect pb
-  apply pa_mul_b.difference pa_gcd_b
+  apply (pa.merge pb).difference (pa.intersect pb)
   apply dvd.trans (nat.gcd.is_dvd a b).left
   apply dvd.mul_left
+
+theorem PrimeFactorization.union.proof
+  (fa: PrimeFactorization a)
+  (fb: PrimeFactorization b)
+  (fab: PrimeFactorization (a.lcm b)):
+  fab.factors = fa.factors.sorted_union fb.factors := by
+  generalize h:PrimeFactorization.union fa fb = fab'
+  rw [Subsingleton.allEq fab fab']
+  rw [←h]
+  unfold union
+  rw [List.sorted.union_def]
+  rfl
+  exact fa.sorted
+  exact fb.sorted
+
+#print axioms PrimeFactorization.union.proof
